ifc-machine/pico/tmu/amach_ni/NIAbstractMachine.v
@@ -56,19 +56,12 @@ Proof.
   eapply success_runSTO_None in H; eauto.
 Qed.
 
-Program Instance AMObservableSemantics : TINI.ObservableSemantics := {
-  state := AS;
-  event := option Event;
-  step := step_rules;
-
-  observer := T;
-  
-  s_equiv := low_equiv_full_state;
-
+Program Instance AMObserableEvent : TINI.ObservableEvent T (option Event) := {
   e_equiv := low_equiv_event;
   e_low := visible_event;
   e_low_dec := visible_event_dec
-}.
+}.  
+
 
 Next Obligation.
   inv H; split; intros H; inv H; auto;
@@ -89,7 +82,14 @@ Next Obligation.
   try solve [constructor (solve [eauto])].
 Qed.
 
-Program Instance AMUnwindingSemantics : TINI.UnwindingSemantics := {
+Program Instance AMObservableSemantics :
+  TINI.ObservableSemantics T (option Event) AS := {
+  step := step_rules;
+  s_equiv := low_equiv_full_state
+}.
+
+Program Instance AMUnwindingSemantics :
+  TINI.UnwindingSemantics (state:=AS) := {
   s_low := low_pc;
   s_low_dec := low_pc_dec
 }.
@@ -153,8 +153,8 @@ Next Obligation.
   eapply highlowstep; eauto.
 Qed.
 
-Theorem noninterference : TINI.tini.
-Proof. apply TINI.noninterference. Qed.
+Theorem noninterference : TINI.tini (state:=AS).
+Proof. apply TINI.noninterference. exact AMUnwindingSemantics. Qed.
 
 (* Theorem lockstep_ni_amach : *)
 (*   lockstep_ni_state_evt step_rules low_pc success low_equiv_full_state. *)
